\section{Sequential Tree Map}

This example is presented for comparison with the parallel tree map given in
chapter 4.
We use \T{int} labelled binary trees.
%
\begin{equation*}
  \T{datatype tree} = \T{E of Unit | N of int$\times$tree$\times$tree}
\end{equation*}
%
Tree \T{map f t} applies the function \T{f} to every label in the tree \T{t}.
%
\begin{align*}
  \T{map} &= \lambda f.\lambda t.\T{rec}(t, \T{E} \mapsto \T{E}, \T{N} \mapsto \LP x,\LP t_0,r_0\RP,\LP t_1,r_1\RP\RP. \T{N}\LP f\ x, \T{force}(r_0), \T{force}(r_1)\RP)
\end{align*}

\subsection{Translation}
%
\begin{align*}
  &\text{We apply the abstraction rule twice.} \\
  \|\T{map}\| &= \LP 0,\lambda f.\LP 0,\lambda t.\|\T{rec}(t, \T{E} \mapsto \T{E},\\
              &\quadsix\T{N} \mapsto \LP x,\LP t_0,r_0\RP,\LP t_1,r_1\RP\RP.\T{N}\LP f\ x,\T{force}(r_0),\T{force}(r_1)\RP)\|\RP\RP \\
              &\text{We apply the recursor translation rule.} \\
              &= \LP 0,\lambda f.\LP 0,\lambda t.\|t\|_c +_c \T{rec}(\|t\|_p, \T{E} \mapsto 1 +_c \|\T{E}\|,\\
              &\quadsix \T{N} \mapsto \LP x,\LP t_0,r_0\RP,\LP t_1,r_1\RP\RP.1 +_c \|\T{N}\LP f\ x,\T{force}(r_0),\T{force}(r_1)\RP\|)\RP\RP \\
  %
              &\text{The translation of the variable $t$ is $\LP 0,t\RP$.} \\
              &\text{The translation of the constructor \T{E} with $\LP\RP$ as its argument is $\LP 0,\T{E}\RP$.} \\
              &\text{The translation of the constructor \T{N}$\LP e\RP$ is $\LP \|e\|_c,\T{N}\LP\|e\|_p\RP\RP$.} \\
  %
              &\text{$f$ and $x$ are variables, so their translations are $\LP 0,f\RP$ and $\LP 0,x\RP$ respectively.}\\
              &\quadthree \|f\ x\| = \LP 1 + \|f\|_c + \|x\|_c +_c \|f\|_p\|x\|_p = \LP 1 + (f\ x)_c,(f\ x)_c\RP \\
              &\text{$r_0$ and $r_1$ are also variables.} \\
              &\quadthree \|\T{force}(r_i)\| = \|r_i\|_c +_c \|r_i\|_p = \LP 0,r_i\RP +_c \LP 0,r_i\RP = r_i \\
  %
              &\text{We use this result to translate the argument to the \T{N} constructor.} \\
              &\quadthree \|\LP f\ x,\T{force}(r_0),\T{force}(r_1)\RP\| = \\
              &\quadsix \LP \|f\ x\|_c + \|\T{force}(r_0)\|_c + \|\T{force}(r_1)\|_c, \\
              &\quadseven \LP \|f\ x\|_p,\|\T{force}(r_0)\|_p\RP,\|\T{force}(r_1)\|_p\RP\RP \\
              &\quadthree = \LP 1 + (f\ x)_c + r_{0c} + r_{1c},\LP (f\ x)_p, r_{0p}, r_{1p}\RP\RP\\
  %
              &\text{We use this to translate the \T{N} constructor.} \\
              &\T{N}\LP f\ x,\T{force}(r_0),\T{force}(r_1)\RP = \LP 1 + (f\ x)_c + r_{0c} + r_{1c}, \T{N}\LP(f\ x)_p,r_{0p},r_{1p}\RP\RP \\
  %
              &\text{We use this to complete the translation of \T{map}.} \\
              &= \LP 0,\lambda f.\LP 0,\lambda t.\T{rec}(t, \T{E} \mapsto \LP 1,\T{E}\RP,\\
              &\quadfive \T{N} \mapsto \LP x,\LP t_0,r_0\RP,\LP t_1,r_1\RP\RP.\LP 2 + (f\ x)_c + r_{0c} + r_{1c}, \T{N}\LP (f\ x)_p,r_{0p},r_{1p}\RP\RP)\RP\RP \\
\end{align*}
%
The translation of \T{map} applied to a function \T{f} and a tree \T{t} is:
%
\begin{align*}
  \|\T{map f t}\| &= (1 + \|\T{map f}\|_c + \|t\|_c) +_c \|\T{map f}\|_p \|t\|_p \\
                  &\qquad \|\T{map f}\| = (1 + \|\T{map}\|_c + \|f\|_c) +_c \|\T{map}\|_p \|f\|_p \\
                  &\text{Since the cost of \T{map} and \T{map f} are $0$, we can simplify this.} \\
                  &\quadfive = \LP 1 + \|f\|_c, (\|\T{map}\|_p \|f\|_p)_p \RP \\
                  &= (2 + \|f\|_c + \|t\|_c) +_c (\|\T{map}\|_p \|f\|_p)_p \|t\|_p
\end{align*}
%

\subsection{Interpretation}
%
We interpret trees as a three-tuple of their largest element and number of
\T{N} constructors.
%
\begin{align*}
  \LB tree \RB &= \mathbb{Z} \times \mathbb{Z} \\
  D_\T{tree} &= \{\ast\} + \mathbb{Z} \times \LB \T{tree} \RB \times \LB \T{tree} \RB \\
  size_\T{tree}(\ast) &= (0, 0) \\
  size_\T{tree}(x, (m_0, n_0), (m_1, n_1)) &= (max(x, m_0, m_1), 1 + n_0 + n_1)
\end{align*}
%
We will interpret the \T{rec} construct first, since it drives the cost of
\T{map}.
%
\begin{align*}
  g(i,n) &= \LB\T{rec}(t, \T{E} \mapsto \LP 1,\T{E}\RP, \\
               &\quad \T{N} \mapsto \LP x,\LP t_0,r_0\RP,\LP t_1,r_1\RP\RP.\LP 2 + (f\ x)_c + r_{0c} + r_{1c}, \T{N}\LP (f\ x)_p,r_{0p},r_{1p}\RP\RP)\RP\RP\RB \xi\\
               &\text{where } \xi = \{t \mapsto (i,n), f \mapsto f \} \\
               &= \bigvee\limits_{size(z) \leq n} case(z, f_E, f_N) \\
               &\text{where} \\
  f_E(\ast) &= \LB \LP 1,\T{E}\RP\RB\xi  \\
            &= (1,(0,0)) \\
  f_N(j,m_0,m_1) &= \LB \LP 2 + (f\ x)_c + r_{0c} + r_{1c}, \T{N}\LP (f\ x)_p,r_{0p},r_{1p}\RP\RP \RB \xi' \\
                 &\text{where } \xi' = \xi \{ x \mapsto j, r_0 \mapsto g(j,m_0), r_1 \mapsto g(j,m_1) \} \\
\end{align*}
%
To obtain a closed form solution for this recurrence, we first eliminate the
big maximum.
%
%\begin{description}
%  \item[if $n=0$]\hfill \\
%    $g(i,0) = \bigvee\limits_{size(z) \leq (i, 0)} case(z, f_E, f_N) = (1,(0,0))$
%  \item[if $n>0$]\hfill \\
%    \begin{align*}
%      g(i,n) &= \bigvee\limits_{size(z) \leq (i,n)} case(z, f_E,f_N) \\
%             &= \bigvee\limits_{size(
%    \end{align*}
%\end{description}
